lib/steel/pulse/Pulse.Elaborate.Pure.fst
@@ -58,7 +58,22 @@ let rec elab_term (top:term)
 
     | Tm_FStar t ->
       w t
-  
+      
+let elab_pat_arg (pi : RT.pp_name_t & bool) : R.pattern & bool =
+  let (v, i) = pi in
+  R.Pat_Var (Sealed.seal RT.tun) v, i
+
+let elab_pat (p:pattern) : Tot R.pattern =
+  let elab_fv (f:fv) : R.fv =
+    R.pack_fv f.fv_name
+  in
+  match p with
+  | Pat_Constant c -> R.Pat_Constant c
+  | Pat_Var v -> R.Pat_Var (Sealed.seal R.(pack_ln Tv_Unknown)) v
+  | Pat_Cons fv vs ->
+    R.Pat_Cons (elab_fv fv) None (L.map elab_pat_arg vs)
+
+let elab_pats (ps:list pattern) : Tot (list R.pattern) = L.map elab_pat ps
 
 let elab_st_comp (c:st_comp)
   : R.universe & R.term & R.term & R.term
