lib/steel/pulse/Pulse.Syntax.Printer.fst
@@ -175,6 +175,10 @@ let rec st_term_to_string' (level:string) (t:st_term)
         (st_term_to_string' (indent level) else_)
         level
 
+    | Tm_Match {sc} ->
+      sprintf "match (%s) with ..."
+        (term_to_string sc)
+
     | Tm_IntroPure { p } ->
       sprintf "introduce pure (\n%s%s)"
         (indent level)
@@ -274,6 +278,7 @@ let tag_of_st_term (t:st_term) =
   | Tm_Bind _ -> "Tm_Bind"
   | Tm_TotBind _ -> "Tm_TotBind"
   | Tm_If _ -> "Tm_If"
+  | Tm_Match _ -> "Tm_Match"
   | Tm_IntroPure _ -> "Tm_IntroPure"
   | Tm_ElimExists _ -> "Tm_ElimExists"
   | Tm_IntroExists _ -> "Tm_IntroExists"
@@ -303,6 +308,7 @@ let rec print_st_head (t:st_term)
   | Tm_Bind _ -> "Bind"
   | Tm_TotBind _ -> "TotBind"
   | Tm_If _ -> "If"
+  | Tm_Match _ -> "Match"
   | Tm_While _ -> "While"
   | Tm_Admit _ -> "Admit"
   | Tm_Par _ -> "Par"
@@ -329,6 +335,7 @@ let rec print_skel (t:st_term) =
   | Tm_Bind { head=e1; body=e2 } -> Printf.sprintf "(Bind %s %s)" (print_skel e1) (print_skel e2)
   | Tm_TotBind { body=e2 } -> Printf.sprintf "(TotBind _ %s)" (print_skel e2)
   | Tm_If _ -> "If"
+  | Tm_Match _ -> "Match"
   | Tm_While _ -> "While"
   | Tm_Admit _ -> "Admit"
   | Tm_Par _ -> "Par"
