share/steel/examples/pulse/MatchBasic.fst
@@ -1,0 +1,100 @@
+module MatchBasic
+
+#set-options "--warn_error -249"
+#set-options "--error_contexts true"
+
+module T = FStar.Tactics
+module PM = Pulse.Main
+open Steel.ST.Util
+open Steel.ST.Reference
+open Steel.FractionalPermission
+open FStar.Ghost
+open Pulse.Steel.Wrapper
+
+```pulse
+fn test1 (n:nat)
+  requires emp
+  returns r:int
+  ensures emp
+{
+  (* let v = n; *)
+  match n {
+    0 -> { 1 }
+    _ -> { 0 }
+  }
+}
+```
+
+```pulse
+fn test2 (n:nat)
+  requires emp
+  returns r:int
+  ensures emp
+{
+  let v = n;
+  match n {
+    0 -> { 1 }
+    x -> { x }
+  }
+}
+```
+
+```pulse
+fn test3 (n:nat)
+  requires emp
+  returns r:int
+  ensures emp
+{
+  match n {
+    0 -> { 1 }
+    x -> { let y = x+1; y }
+  }
+}
+
+```
+
+// FIXME: Need to qualifiy the constructors or otherwise they desugar to
+// the (not yet in scope) type below.
+```pulse
+fn test3_5 (n:option int) (z:bool)
+  requires emp
+  returns r:int
+  ensures emp
+{
+  match n {
+    Pervasives.None -> { (-1) }
+    Pervasives.Some x -> { x }
+  }
+}
+```
+
+noeq
+type optionint =
+  | None
+  | Some of int
+
+```pulse
+fn test4 (n:optionint) (z:bool)
+  requires emp
+  returns r:int
+  ensures emp
+{
+  match n {
+    MatchBasic.None -> { 0 }
+    MatchBasic.Some x -> { x }
+  }
+}
+```
+
+```pulse
+fn test5 (n:option int) (z:bool)
+  requires emp
+  returns r:int
+  ensures emp
+{
+  match n {
+    Pervasives.None -> { (-1) }
+    Pervasives.Some x -> { x }
+  }
+}
+```
